Updates in old/Pred.v

old/Pred.v
@@ -3,7 +3,6 @@ Require Import
   Coq.Logic.PropExtensionality
   Hask.Control.Monad
   Data.Either
-  Pact.ilist
   Pact.Lib
   Pact.Ty
   Pact.Exp
@@ -31,129 +30,90 @@ Import ListNotations.
 
 Section Pred.
 
-Definition env   : Type := PactEnv.
 Definition state : Type := PactState.
-Definition log   : Type := PactLog.
 
-Definition rprop   : Type := env → Prop.
-Definition sprop   : Type := state → Prop.
+Definition hprop   : Type := state → Prop.
+Definition vprop τ : Type := SemTy (m:=PactM) τ → hprop.
 Definition eprop   : Type := Err → Prop.
-Definition vprop τ : Type := SemTy (m:=PactM) τ → sprop.
 
-Implicit Type G : rprop.
-Implicit Type H : sprop.
+Implicit Type H : hprop.
 Implicit Type Z : eprop.
 
-Definition hoare G H `(e : expM τ) (Q : vprop τ) Z : Prop :=
-  ∀ (r : env), G r →
+Definition hoare H `(e : expM τ) (Q : vprop τ) Z : Prop :=
   ∀ (s : state), H s ->
-  match e r s : Err + ⟦τ⟧ * (state * _) with
-  | inr (v, (s', _)) => Q v s'
+  match e s : Err + ⟦τ⟧ * state with
+  | inr (v, s') => Q v s'
   | inl err => Z err
   end.
 
 Declare Scope pred_scope.
 Open Scope pred_scope.
 
-Notation "{ G & H } x ← e { Q | Z }" :=
-  (hoare G H e (λ x, Q) Z) (at level 1, e at next level) : pred_scope.
+Notation "{{ H }} x ← e { Q | Z }" :=
+  (hoare H e (λ x, Q) Z) (at level 1, e at next level) : pred_scope.
 
 #[local] Hint Unfold hoare : core.
 
-Theorem hoare_post_true G H `(Q : vprop τ) Z e :
+Theorem hoare_post_true H `(Q : vprop τ) Z e :
   (∀ v s, Q v s) →
   (∀ err, Z err) →
-  { G & H } x ← e { Q x | Z }.
+  {{H}} x ← e {Q x|Z}.
 Proof.
   unfold hoare; sauto.
 Qed.
 
-Theorem hoare_pre_false G H `(Q : vprop τ) Z e :
-  (∀ r, ¬ (G r)) ∨ (∀ s, ¬ (H s)) →
-  { G & H } x ← e { Q x | Z }.
+Theorem hoare_pre_false H `(Q : vprop τ) Z e :
+  (∀ s, ¬ (H s)) →
+  {{H}} x ← e {Q x|Z}.
 Proof.
   unfold hoare; sauto.
 Qed.
 
-Definition sprop_conj (H H' : sprop) : sprop :=
+Definition hprop_conj (H H' : hprop) : hprop :=
   λ st, H st ∧ H' st.
 
-Arguments sprop_conj _ _ /.
+Arguments hprop_conj _ _ /.
 
-#[local] Hint Unfold sprop_conj : core.
+#[local] Hint Unfold hprop_conj : core.
 
-Notation "Q \∧ H" := (sprop_conj Q H) (at level 10) : pred_scope.
+Notation "Q \∧ H" := (hprop_conj Q H) (at level 10) : pred_scope.
 
-Definition quintuple
-  (G : rprop)
-  (H : sprop)
+Definition quadruple
+  (H : hprop)
   `(e : expM τ)
   (Q : vprop τ)
   (Z : eprop) : Prop :=
-  ∀ H', { G & H \∧ H' } x ← e { Q x \∧ H' | Z }.
+  ∀ H', {{ H \∧ H' }} x ← e { Q x \∧ H' | Z }.
 
-#[local] Hint Unfold quintuple : core.
+#[local] Hint Unfold quadruple : core.
 
-Theorem frame_rule {G H} `{e : expM τ} {Q Z H'} :
-  quintuple G H e Q Z →
-  quintuple G (H \∧ H') e (λ x, Q x \∧ H') Z.
+Theorem frame_rule {H} `{e : expM τ} {Q : vprop τ} {Z H'} :
+  quadruple H e Q Z →
+  quadruple (H \∧ H') e (λ x, Q x \∧ H') Z.
 Proof.
-  unfold quintuple, hoare.
+  unfold quadruple, hoare.
   intros.
-  destruct H2, H2.
-  pose proof (H0 _ _ H1 _ (conj H2 H4)).
-  pose proof (H0 _ _ H1 _ (conj H2 H3)).
+  destruct H1, H1.
+  pose proof (H0 _ _ (conj H1 H3)).
+  pose proof (H0 _ _ (conj H1 H2)).
   sauto lq: on.
 Qed.
 
 Definition WP : Type :=
-  ∀ τ (e : expM τ) (Q : vprop τ) (Z : eprop), env → sprop.
+  ∀ τ (e : expM τ) (Q : vprop τ) (Z : eprop), hprop.
 
-Definition wp
-  `(e : expM τ)
-  (Q : vprop τ)
-  (Z : eprop) : sprop :=
-  λ st,
-    ∃ r (G : rprop) (H : sprop),
-      G r ∧ (H \∧ (λ _, quintuple G H e Q Z) st).
+Definition wp `(e : expM τ) (Q : vprop τ) (Z : eprop) : hprop :=
+  λ st, ∃ (H : hprop), (H \∧ (λ _, quadruple H e Q Z) st).
 
 #[local] Hint Unfold wp : core.
 
-Definition himpl (P Q : sprop) : Prop :=
+Definition himpl (P Q : hprop) : Prop :=
   ∀ s, P s → Q s.
 
 #[local] Hint Unfold himpl : core.
 
 Notation "P ==> Q" :=
   (himpl P Q) (at level 55, Q at level 55) : pred_scope.
-
-Definition hrimpl (G : rprop) (P : sprop) (Q : env → sprop) : Prop :=
-  ∀ r s, G r → P s → Q r s.
-
-#[local] Hint Unfold hrimpl : core.
-
-Notation "P =[ G ]=> Q" :=
-  (hrimpl G P Q) (at level 55, G at level 55, Q at level 55) : pred_scope.
-
-Lemma dehrimpl `(H : P =[ G ]=> Q) : ∀ r, G r → P ==> Q r.
-Proof.
-  unfold himpl, hrimpl in *.
-  intuition.
-Defined.
-
-Lemma hrimplize `(H : ∀ r, G r → P ==> Q r) : P =[ G ]=> Q.
-Proof.
-  unfold himpl, hrimpl in *.
-  intuition.
-Defined.
-
-Corollary dehrimpl_hrimplize `(H : ∀ r, G r → P ==> Q r) :
-  dehrimpl (hrimplize H) = H.
-Proof. reflexivity. Qed.
-
-Corollary hrimplize_dehrimpl `(H : P =[ G ]=> Q) :
-  hrimplize (dehrimpl H) = H.
-Proof. reflexivity. Qed.
 
 Definition vimpl {τ} (Q R : vprop τ) : Prop :=
   ∀ v, Q v ==> R v.
@@ -162,18 +122,17 @@ Definition vimpl {τ} (Q R : vprop τ) : Prop :=
 
 Notation "Q ===> R" := (vimpl Q R) (at level 55) : pred_scope.
 
-Theorem wp_equiv {G H} `{e : expM τ} {Q Z} :
-  (H ==> wp e Q Z) ↔ (quintuple G H e Q Z).
+Theorem wp_equiv {H} `{e : expM τ} {Q : vprop τ} {Z} :
+  (H ==> wp e Q Z) ↔ (quadruple H e Q Z).
 Proof.
-  unfold hrimpl, wp, quintuple, hoare, sprop_conj.
+  unfold wp, quadruple, hoare, hprop_conj.
   split; intros.
   - reduce.
-    specialize (H0 _ H2).
+    specialize (H0 _ H1).
     simpl in H0.
     reduce.
-    unshelve epose proof (H5 _ _ H0 _ (conj _ H3)); auto.
-  - exists G.
-    exists H.
+    unshelve epose proof (H3 _ _ (conj _ H2)); auto.
+  - exists H.
     split; auto.
 Qed.
 
@@ -211,10 +170,10 @@ Proof.
 Qed.
 
 Theorem wp_unique (wp1 wp2 : WP) :
-  (∀ G H τ (e : expM τ) Q Z,
-     quintuple G H e Q Z ↔ H =[G]=> wp1 _ e Q Z) →
-  (∀ G H τ (e : expM τ) Q Z,
-     quintuple G H e Q Z ↔ H =[G]=> wp2 _ e Q Z) →
+  (∀ H τ (e : expM τ) (Q : vprop τ) Z,
+     quadruple H e Q Z ↔ H ==> wp1 _ e Q Z) →
+  (∀ H τ (e : expM τ) (Q : vprop τ) Z,
+     quadruple H e Q Z ↔ H ==> wp2 _ e Q Z) →
   wp1 = wp2.
 Proof.
   intros.
@@ -222,36 +181,31 @@ Proof.
   extensionality e.
   extensionality Q.
   extensionality Z.
-  extensionality r.
   apply himpl_antisym.
-  - destruct (H0 (λ r', r = r') (wp1 τ e Q Z r) τ e Q Z) as [H5 H6]; clear H0.
-    eapply dehrimpl in H5; eauto.
-    apply H; intros.
-    subst.
-    apply hrimplize; intros; subst.
+  - destruct (H0 (wp1 τ e Q Z) τ e Q Z) as [H5 H6]; clear H0.
+    apply H5; intros.
+    apply H.
     reflexivity.
-  - destruct (H (λ r', r = r') (wp2 τ e Q Z r) τ e Q Z) as [H5 H6]; clear H.
-    eapply dehrimpl in H5; eauto.
-    apply H0; intros.
-    subst.
-    apply hrimplize; intros; subst.
+  - destruct (H (wp2 τ e Q Z) τ e Q Z) as [H5 H6]; clear H.
+    apply H5; intros.
+    apply H0.
     reflexivity.
 Qed.
 
-Theorem quintuple_conseq {G τ} {e : expM τ} {H' Q' H Q Z} :
-  quintuple G H' e Q' Z →
+Theorem quadruple_conseq {τ} {e : expM τ} {H' H} {Q' Q : vprop τ} {Z} :
+  quadruple H' e Q' Z →
   H ==> H' →
   Q' ===> Q →
-  quintuple G H e Q Z.
+  quadruple H e Q Z.
 Proof.
   intros.
   repeat intro.
-  destruct H4.
-  specialize (H1 _ H4).
-  specialize (H0 H'0 _ H3 _ (conj H1 H5)).
+  destruct H3.
+  specialize (H1 _ H3).
+  specialize (H0 _ _ (conj H1 H4)).
   matches.
   reduce.
-  unfold sprop_conj in *.
+  unfold hprop_conj in *.
   intuition.
 Qed.
 
@@ -260,30 +214,24 @@ Program Instance vimpl_PreOrder {τ} : PreOrder (vimpl (τ:=τ)).
 Next Obligation. now apply H0, H. Qed.
 
 Theorem wp_from_weakest_pre (wp' : WP) :
-  (∀ G H τ (e : expM τ) Q Z r,
-     quintuple G (wp' _ e Q Z r) e Q Z) →          (* wp_pre *)
-  (∀ G H τ (e : expM τ) Q Z,
-     quintuple G H e Q Z → ∀ r, G r → H ==> wp' _ e Q Z r) → (* wp_weakest *)
-  (∀ G H τ (e : expM τ) Q Z,
-     ∀ r, G r → H ==> wp' _ e Q Z r ↔ quintuple G H e Q Z).  (* wp_equiv *)
+  (∀ H τ (e : expM τ) (Q : vprop τ) Z,
+     quadruple (wp' _ e Q Z) e Q Z) →          (* wp_pre *)
+  (∀ H τ (e : expM τ) (Q : vprop τ) Z,
+     quadruple H e Q Z → H ==> wp' _ e Q Z) → (* wp_weakest *)
+  (∀ H τ (e : expM τ) (Q : vprop τ) Z,
+     H ==> wp' _ e Q Z ↔ quadruple H e Q Z).  (* wp_equiv *)
 Proof.
   intros M1 M2.
   split; intro M.
-  - eapply quintuple_conseq; eauto.
+  - eapply quadruple_conseq; eauto.
   - eapply M2; eauto.
 Qed.
 
-#[local] Hint Unfold RWSE_join : core.
-#[local] Hint Unfold RWSE_ap : core.
-#[local] Hint Unfold Either_map : core.
-#[local] Hint Unfold Tuple.first : core.
-#[local] Hint Unfold Basics.compose : core.
-#[local] Hint Unfold Datatypes.id : core.
-
 Notation "e =====> e'" :=
-  (∀ Q Z r, wp e Q Z r ==> wp e' Q Z r) (at level 100, e' at next level) : pred_scope.
+  (∀ Q Z, wp e Q Z ==> wp e' Q Z) (at level 100, e' at next level) : pred_scope.
 
-Lemma eval_if_trm (t0 : Exp [] 𝔹) v0 {τ} (t1 t2 : Exp [] τ) (v : SemTy τ) s s' s'' :
+Lemma eval_if_trm (t0 : Exp [] 𝔹) v0 {τ} (t1 t2 : Exp [] τ)
+  (v : SemTy τ) s s' s'' :
   t0 ~[s => s']~> v0 →
   If (Lit (LitBool v0)) t1 t2 ~[s' => s'']~> v →
   If t0 t1 t2 ~[s => s'']~> v.
@@ -291,35 +239,33 @@ Proof.
   unfold eval.
   intros.
   simp SemExp in *; simpl in *; autounfold in *.
-  specialize (H r).
-  specialize (H0 r).
-  reduce.
-  rewrite H.
-  sauto.
+  now rewrite H.
 Qed.
 
-Lemma hoare_if G H (b : Exp [] 𝔹) τ (t1 t2 : Exp [] τ) Q Q' Z :
-  hoare G H ⟦b⟧ Q' Z →
-  (∀ v, hoare G (Q' v) ⟦If (Lit (LitBool v)) t1 t2⟧ Q Z) →
-  hoare G H ⟦If b t1 t2⟧ Q Z.
+Lemma hoare_if H (b : Exp [] 𝔹) τ (t1 t2 : Exp [] τ)
+  (Q' : vprop 𝔹) (Q : vprop τ) Z :
+  hoare H ⟦b⟧ Q' Z →
+  (∀ v, hoare (Q' v) ⟦If (Lit (LitBool v)) t1 t2⟧ Q Z) →
+  hoare H ⟦If b t1 t2⟧ Q Z.
 Proof.
   autounfold.
   repeat intro.
   simp SemExp in *; simpl in *; autounfold in *.
-  specialize (H0 _ H2 _ H3).
-  destruct (⟦b⟧ _ _) eqn:Heqe; auto.
+  specialize (H0 _ H2).
+  destruct (⟦b⟧ _) eqn:Heqe; auto.
   reduce.
-  specialize (H1 _ _ H2 _ H0).
+  specialize (H1 _ _ H0).
   simp SemExp in *; simpl in *; autounfold in *.
-  sauto lq: on.
+  exact H1.
 Qed.
 
-Lemma quintuple_if G H (b : Exp [] 𝔹) τ (t1 t2 : Exp [] τ) Q Q' Z :
-  quintuple G H ⟦b⟧ Q' Z →
-  (∀ v, quintuple G (Q' v) ⟦If (Lit (LitBool v)) t1 t2⟧ Q Z) →
-  quintuple G H ⟦If b t1 t2⟧ Q Z.
+Lemma quadruple_if H (b : Exp [] 𝔹) τ (t1 t2 : Exp [] τ)
+  (Q' : vprop 𝔹) (Q : vprop τ) Z :
+  quadruple H ⟦b⟧ Q' Z →
+  (∀ v, quadruple (Q' v) ⟦If (Lit (LitBool v)) t1 t2⟧ Q Z) →
+  quadruple H ⟦If b t1 t2⟧ Q Z.
 Proof.
-  unfold quintuple.
+  unfold quadruple.
   intros.
   eapply hoare_if; eauto.
   intros.
@@ -328,63 +274,62 @@ Qed.
 
 Ltac wp r H :=
   intros;
-  apply (dehrimpl (G:=λ r', r = r')); eauto;
   eapply wp_equiv;
   eapply H; eauto;
   eapply wp_equiv;
-  apply hrimplize; intros;
   subst; reflexivity.
 
 (* An if statement simply propagates the environment. *)
-Corollary wp_if (b : Exp [] 𝔹) τ (t1 t2 : Exp [] τ) Q Z :
+Corollary wp_if (b : Exp [] 𝔹) τ (t1 t2 : Exp [] τ) (Q : vprop τ) Z :
   wp ⟦b⟧ (λ v, wp ⟦If (Lit (LitBool v)) t1 t2⟧ Q Z) Z
     ==> wp ⟦If b t1 t2⟧ Q Z.
 Proof.
   unfold wp.
   simpl.
   repeat intro.
-  destruct H as [G [H [HG [HH H0]]]].
-  exists G, H.
-  do 2 (split; auto).
-  eapply quintuple_if; eauto.
-  intros.
+  destruct H as [H [HH H0]].
+  exists H.
+  split; auto.
+  eapply quadruple_if; eauto; intros.
   simpl.
-  unfold quintuple, hoare in *.
+  unfold quadruple, hoare in *.
   intros.
   simpl in *.
   reduce.
-  specialize (H0 _ _ H1 _ (conj HH HH)).
-  destruct (⟦b⟧ _ _); simp SemExp in *; simpl in *; autounfold in *.
-  - specialize (H5 _ _ H2 _ (conj H4 H3)).
-    destruct v.
-    apply H5.
-
-  specialize (H0 H').
-
-  unshelve eapply quintuple_conseq; eauto.
-    admit.
+  specialize (H0 _ _ (conj HH HH)).
+  destruct (⟦b⟧ _);
+  simp SemExp in *; simpl in *;
+  unravel; reduce;
+  exact (H3 _ _ (conj H1 H2)).
 Qed.
 
-Lemma quintuple_app_fun G H `(v : Exp [] dom) x `(e : Exp [dom] cod) Q Z :
-  ⟦v⟧ = pure x →
-  quintuple G H ⟦ (x, tt) ⊨ e ⟧ Q Z →
-  quintuple G H ⟦APP (LAM e) v⟧ Q Z.
+Lemma quadruple_app_fun H `(v : Exp [] dom) x `(e : Exp [dom] cod)
+  (Q : vprop cod) Z :
+  (∀ s, v ~[ s => s ]~> x) →
+  quadruple H ⟦ (x, tt) ⊨ e ⟧ Q Z →
+  quadruple H ⟦APP (LAM e) v⟧ Q Z.
 Proof.
   intros.
+  repeat intro.
+  specialize (H1 _ _ H2).
+  simpl in *.
   erewrite sem_app_lam; eauto.
 Qed.
 
 Lemma wp_app_fun `(v : Exp [] dom) x `(e : Exp [dom] cod) :
-  ⟦v⟧ = pure x →
+  (∀ s, v ~[ s => s ]~> x) →
   ⟦ (x, tt) ⊨ e ⟧ =====> ⟦APP (LAM e) v⟧.
-Proof. wp r quintuple_app_fun. Qed.
+Proof. wp r quadruple_app_fun. Qed.
 
-Equations wpc `(e : Exp [] τ) (Q : vprop τ) Z : env → sprop :=
+(*
+Equations wpc `(e : Exp [] τ) (Q : vprop τ) Z : hprop :=
+  wpc (Lit l) Q Z := Q (SemLit l);
   wpc (APP f v) Q Z := wp ⟦APP f v⟧ Q Z;
-  wpc (Seq e1 e2) Q Z := λ r, wpc e1 (λ v, wpc e2 Q Z r) Z r;
-  wpc (If (Lit (LitBool b)) t e) Q Z :=
-    if b then wpc t Q Z else wpc e Q Z;
+  wpc (Seq e1 e2) Q Z := wpc e1 (λ _, wpc e2 Q Z) Z;
+  wpc (If b t e) Q Z :=
+    wpc b (λ b', if b' then wpc t Q Z else wpc e Q Z) Z;
   wpc _ Q Z := _.
+*)
 
 (* This encodes a boolean predicate in positive normal form. *)
 Inductive Pred Γ : ∀ {τ}, Γ ⊢ τ → Set :=
